Update on 7 December 2012.

theories/core/utp_value.thy
@@ -1,16 +1,16 @@
 (******************************************************************************)
 (* Project: Unifying Theories of Programming in HOL                           *)
 (* File: utp_value.thy                                                        *)
-(* Author: Frank Zeyda, University of York (UK)                               *)
+(* Authors: Frank Zeyda & Simon Foster, University of York (UK)               *)
 (******************************************************************************)
 
-header {* Abstract Values *}
+header {* Value Locales *}
 
 theory utp_value
-imports "../utp_common"
+imports "../utp_common" utp_sorts utp_types
 begin
 
-subsection {* Locale @{term "VALUE"} *}
+subsection {* Abstract Values *}
 
 locale VALUE =
 -- {* Typing Relation *}
@@ -24,7 +24,28 @@ subsection {* Universe *}
 definition VALUE :: "'VALUE set" where
 "VALUE = UNIV"
 
-subsection {* Carrier Set *}
+subsection {* Well-formed Values *}
+
+definition WF_VALUE :: "'VALUE set" where
+"WF_VALUE = {v . \<exists> t . v : t}"
+
+theorem WF_VALUE_non_empty :
+"WF_VALUE \<noteq> {}"
+apply (simp add: WF_VALUE_def)
+apply (insert type_non_empty)
+apply (drule_tac x = "t" in meta_spec)
+apply (clarify)
+apply (rule_tac x = "x" in exI)
+apply (rule_tac x = "t" in exI)
+apply (assumption)
+done
+
+theorem WF_VALUE_member :
+"(x \<in> WF_VALUE) \<longleftrightarrow> (\<exists> t . x : t)"
+apply (simp add: WF_VALUE_def)
+done
+
+subsection {* Carrier Sets *}
 
 definition carrier :: "'TYPE \<Rightarrow> 'VALUE set" where
 "carrier t = {x . x : t}"
@@ -35,18 +56,69 @@ apply (simp add: carrier_def type_non_empty)
 done
 
 theorem carrier_member :
-"x : t \<Longrightarrow> x \<in> carrier t"
+"x \<in> (carrier t) \<longleftrightarrow> (x : t)"
 apply (simp add: carrier_def)
 done
 
-theorem carrier_intro :
-"(x : t) = (x \<in> carrier t)"
+theorem carrier_intro [intro] :
+"(x : t) \<Longrightarrow> (x \<in> carrier t)"
 apply (simp add: carrier_def)
 done
 
-theorem carrier_elim :
-"(x \<in> carrier t) = (x : t)"
+theorem carrier_dest [dest] :
+"(x \<in> carrier t) \<Longrightarrow> (x : t)"
 apply (simp add: carrier_def)
+done
+
+theorem WF_VALUE_carrier_member [intro] :
+"x \<in> carrier t \<Longrightarrow> x \<in> WF_VALUE"
+apply (simp add: WF_VALUE_member)
+apply (simp add: carrier_def)
+apply (rule_tac x = "t" in exI)
+apply (assumption)
+done
+
+subsection {* Type Set Carriers *}
+
+definition carrier_types :: "'TYPE set \<Rightarrow> 'VALUE set" where
+"carrier_types ts = \<Union> {carrier t | t . t \<in> ts}"
+
+theorem carrier_types_member :
+"x \<in> (carrier_types ts) \<longleftrightarrow> (\<exists> t \<in> ts . x \<in> carrier t)"
+apply (simp add: carrier_types_def)
+apply (safe)
+apply (rule_tac x = "t" in bexI)
+apply (assumption)+
+apply (rule_tac x = "carrier t" in exI)
+apply (simp)
+apply (rule_tac x = "t" in exI)
+apply (simp)
+done
+
+theorem carrier_types_monotonic :
+"ts1 \<subseteq> ts2 \<Longrightarrow> (carrier_types ts1) \<subseteq> (carrier_types ts2)"
+apply (simp add: carrier_types_def)
+apply (clarsimp)
+apply (rule_tac x = "carrier t" in exI)
+apply (simp)
+apply (rule_tac x = "t" in exI)
+apply (simp)
+apply (auto)
+done
+
+theorem WF_VALUE_carrier_types_member [intro] :
+"x \<in> carrier_types ts \<Longrightarrow> x \<in> WF_VALUE"
+apply (simp add: carrier_types_member)
+apply (clarify)
+apply (erule WF_VALUE_carrier_member)
+done
+
+theorem WF_VALUE_carrier_types :
+"WF_VALUE = carrier_types UNIV"
+apply (simp add: set_eq_iff)
+apply (simp add: WF_VALUE_member)
+apply (simp add: carrier_types_member)
+apply (simp add: carrier_member)
 done
 
 subsection {* Value Sets *}
@@ -65,5 +137,52 @@ theorem set_type_rel_insert [simp] :
 "(insert x s) :\<subseteq> t \<longleftrightarrow> (x : t \<and> s :\<subseteq> t)"
 apply (simp add: set_type_rel_def)
 done
+
+subsection {* Default Value *}
+
+definition SomeValue :: "'TYPE \<Rightarrow> 'VALUE" where
+"SomeValue t = (SOME x . x : t)"
+
+theorem SomeValue_well_typed [simp] :
+"(SomeValue t) : t"
+apply (insert type_non_empty [where t = "t"])
+apply (simp add: SomeValue_def)
+apply (erule someI_ex)
+done
+end
+
+subsection {* Bottom Values *}
+
+locale BOT_VALUE =
+  VALUE "type_rel"
+-- {* Additional constraints are imposed via sort membership. *}
+for type_rel :: "'VALUE :: BOT_SORT \<Rightarrow> 'TYPE \<Rightarrow> bool" (infix ":" 50) +
+assumes bot_type [typing] : "bot : t"
+
+subsection {* Boolean Values *}
+
+locale BOOL_VALUE =
+  BOT_VALUE "type_rel"
+-- {* Additional constraints are imposed via sort membership. *}
+for type_rel :: "'VALUE :: {BOOL_SORT, BOT_SORT} \<Rightarrow>
+    'TYPE :: BOOL_TYPE \<Rightarrow> bool" (infix ":" 50) +
+  assumes TypeLink : "\<And> x. \<lbrakk>\<D> x\<rbrakk> \<Longrightarrow> x : BoolType \<longleftrightarrow> x \<in> range MkBool"
+begin
+
+theorem MkBool_type [typing] :
+"MkBool x : BoolType"
+  by (simp add: Defined TypeLink)
+
+theorem in_range_MkBool :
+"\<lbrakk>x : BoolType; \<D> x\<rbrakk> \<Longrightarrow> x \<in> range MkBool"
+  by (simp add: TypeLink)
+
+theorem MkBool_cases :
+"\<lbrakk>x : BoolType; \<D> x\<rbrakk> \<Longrightarrow> x = MkBool True \<or> x = MkBool False"
+  by (metis (full_types) in_range_MkBool DestBool_inverse)
+
+theorem DestBool_inverse :
+"\<lbrakk>x : BoolType; \<D> x\<rbrakk> \<Longrightarrow> MkBool (DestBool x) = x"
+  by (metis in_range_MkBool DestBool_inverse)
 end
 end
