theories/utp_global.thy
@@ -7,12 +7,14 @@
 header {* Global Syntax *}
 
 theory utp_global
-imports utp_common "core/utp_synonyms"
+imports utp_common "core/utp_synonyms" "core/utp_value"
 begin
 
-text {* This theory introduces generic constants for global syntax. *}
+subsection {* Global Syntax *}
 
-subsection {* Value Syntax *}
+text {* We introduce generic constants for global syntax. *}
+
+subsubsection {* Value Syntax *}
 
 consts global_type_rel :: "'VALUE \<Rightarrow> 'TYPE \<Rightarrow> bool"
 notation global_type_rel (infix ":" 50)
@@ -20,26 +22,26 @@ notation global_type_rel (infix ":" 50)
 consts global_set_type_rel :: "'VALUE set \<Rightarrow> 'TYPE \<Rightarrow> bool"
 notation global_set_type_rel (infix ":\<subseteq>" 50)
 
-subsection {* Predicate Syntax *}
+subsubsection {* Predicate Syntax *}
 
 text {*
   We do not define generic constants for the following two operators. The
   reason for this is that typing can become subtle with generic constants
   here. Namely, it is not enough to type the operand in order to fully type
   the operator. This can lead to unexpected behaviours during parsing; that
-  is, for instance, instantiation of the operators with the wrong types.
+  is, for instance, instantiation of the operators with wrong types. A
+  common solution to this problem is to parametrise the operator in terms of
+  the result type using @{type "itself"}. But this might be too cumbersome.
 *}
-
-text {* TODO: I cannot quite follow the above anymore, review this! *}
 
 (*
 consts global_alphabet ::
-  "('VALUE, 'TYPE) ALPHA_PREDICATE \<Rightarrow>
-   ('TYPE ALPHABET)" ("\<alpha>")
+  "'PREDICATE \<Rightarrow>
+  ('TYPE ALPHABET)" ("\<alpha>")
 
 consts global_predicate ::
-  "('VALUE, 'TYPE) ALPHA_PREDICATE \<Rightarrow>
-   ('VALUE, 'TYPE) PREDICATE ("\<pi>")
+  "'PREDICATE1 \<Rightarrow>
+  ('VALUE, 'TYPE) PREDICATE2 ("\<pi>")
 *)
 
 consts global_binding_equiv ::
@@ -160,6 +162,115 @@ consts Refinement ::
    'PREDICATE \<Rightarrow> bool"
   (infix "\<sqsubseteq>" 50)
 
-subsection {* Relation Syntax *}
+subsubsection {* Relation Syntax *}
 
+subsection {* Global Definitions *}
+
+subsubsection {* Well-formed Values *}
+
+definition WF_VALUE_GLOBAL ::
+  "('VALUE\<Rightarrow> 'TYPE \<Rightarrow> bool) \<Rightarrow> 'VALUE set" where
+"WF_VALUE_GLOBAL type_rel = {v . \<exists> t . type_rel v t}"
+
+notation WF_VALUE_GLOBAL ("WF'_VALUE[_]")
+
+theorem WF_VALUE_GLOBAL_non_empty :
+"VALUE type_rel \<Longrightarrow> WF_VALUE[type_rel] \<noteq> {}"
+apply (simp add: WF_VALUE_GLOBAL_def)
+apply (simp add: VALUE_def)
+apply (drule_tac x = "t" in spec)
+apply (clarify)
+apply (rule_tac x = "x" in exI)
+apply (rule_tac x = "t" in exI)
+apply (assumption)
+done
+
+theorem WF_VALUE_GLOBAL_member :
+"(x \<in> WF_VALUE[type_rel]) \<longleftrightarrow> (\<exists> t . type_rel x t)"
+apply (simp add: WF_VALUE_GLOBAL_def)
+done
+
+(* The commented out stuff below is probably redundant. Remove! *)
+
+(*
+subsubsection {* Carrier Sets *}
+
+definition global_carrier ::
+  "('VALUE \<Rightarrow> 'TYPE \<Rightarrow> bool) \<Rightarrow> 'TYPE \<Rightarrow>  ('VALUE set)" where
+"global_carrier type_rel t = {x . type_rel x t}"
+
+notation global_carrier ("carrier[_]")
+
+theorem global_carrier_member :
+"x \<in> (carrier[type_rel] t) \<longleftrightarrow> (type_rel x t)"
+apply (simp add: global_carrier_def)
+done
+
+theorem global_equals_local_carrier :
+"VALUE type_rel \<Longrightarrow>
+ carrier[type_rel] = VALUE.carrier type_rel"
+apply (rule ext)
+apply (simp add: global_carrier_def)
+apply (simp add: VALUE.carrier_def)
+done
+
+theorem local_equals_global_carrier :
+"VALUE type_rel \<Longrightarrow>
+ VALUE.carrier type_rel = carrier[type_rel]"
+apply (rule ext)
+apply (simp add: VALUE.carrier_def)
+apply (simp add: global_carrier_def)
+done
+*)
+
+(*
+subsubsection {* Type Set Carriers *}
+
+definition global_carrier_types ::
+  "('VALUE \<Rightarrow> 'TYPE \<Rightarrow> bool) \<Rightarrow> ('TYPE set) \<Rightarrow> ('VALUE set)" where
+"global_carrier_types type_rel ts =
+ \<Union> {carrier[type_rel] t | t . t \<in> ts}"
+
+notation global_carrier_types ("carrier'_types[_]")
+
+theorem global_carrier_types_member :
+"x \<in> (carrier_types[type_rel] ts) \<longleftrightarrow>
+ (\<exists> t \<in> ts . x \<in> carrier[type_rel] t)"
+apply (simp add: global_carrier_types_def)
+apply (safe)
+apply (rule_tac x = "t" in bexI)
+apply (assumption)+
+apply (rule_tac x = "carrier[type_rel] t" in exI)
+apply (simp)
+apply (rule_tac x = "t" in exI)
+apply (simp)
+done
+
+theorem global_carrier_types_UNIV :
+"type_rel x t \<Longrightarrow> x \<in> (carrier_types[type_rel] UNIV)"
+apply (simp add: global_carrier_types_member)
+apply (rule_tac x = "t" in exI)
+apply (simp add: global_carrier_member)
+done
+
+theorem global_carrier_types_monotonic :
+"ts1 \<subseteq> ts2 \<Longrightarrow>
+ (carrier_types[type_rel] ts1) \<subseteq> (carrier_types[type_rel] ts2)"
+apply (simp add: global_carrier_types_def)
+apply (clarsimp)
+apply (rule_tac x = "carrier[type_rel] t" in exI)
+apply (simp)
+apply (rule_tac x = "t" in exI)
+apply (simp)
+apply (auto)
+done
+
+theorem WF_VALUE_GLOBAL_carrier_types :
+"WF_VALUE[type_rel] = carrier_types[type_rel] UNIV"
+apply (simp add: set_eq_iff)
+apply (simp add: WF_VALUE_GLOBAL_member)
+apply (simp add: global_carrier_types_member)
+apply (simp add: global_carrier_member)
+done
+*)
 end
